src/program_logic/recovery_adequacy.v
@@ -3,6 +3,146 @@ From iris.algebra Require Import gmap auth agree gset coPset.
 From iris.base_logic.lib Require Import wsat.
 From iris.program_logic Require Export weakestpre.
 From Perennial.program_logic Require Export crash_lang crash_weakestpre.
+Import uPred.
+
+Section crash_adequacy.
+Context `{!irisG Λ Σ}.
+Implicit Types e : expr Λ.
+Implicit Types P Q : iProp Σ.
+Implicit Types Φ : val Λ → iProp Σ.
+Implicit Types Φs : list (val Λ → iProp Σ).
+
+Notation wptp s t := ([∗ list] ef ∈ t, WPC ef @ s; ⊤; ∅ {{ fork_post }} {{ True }})%I.
+
+Lemma wpc_step s e1 σ1 κ κs e2 σ2 efs m Φ Φc :
+  prim_step e1 σ1 κ e2 σ2 efs →
+  state_interp σ1 (κ ++ κs) m -∗ WPC e1 @ s; ⊤; ∅ {{ Φ }} {{ Φc }} ={⊤,∅}▷=∗
+  state_interp σ2 κs (length efs + m) ∗
+  WPC e2 @ s; ⊤; ∅ {{ Φ }} {{ Φc }} ∗
+  wptp s efs.
+Proof.
+  rewrite {1}wpc_unfold /wpc_pre. iIntros (?) "Hσ H".
+  rewrite (val_stuck e1 σ1 κ e2 σ2 efs) //.
+  iDestruct "H" as "(H&_)".
+  iMod ("H" $! σ1 with "Hσ") as "(_ & H)".
+  iMod ("H" $! e2 σ2 efs with "[//]") as "H".
+  by iIntros "!> !>".
+Qed.
+
+Lemma wptp_step s e1 t1 t2 κ κs σ1 σ2 Φ Φc :
+  step (e1 :: t1,σ1) κ (t2, σ2) →
+  state_interp σ1 (κ ++ κs) (length t1) -∗ WPC e1 @ s; ⊤; ∅ {{ Φ }} {{ Φc }}-∗ wptp s t1 ==∗
+  ∃ e2 t2', ⌜t2 = e2 :: t2'⌝ ∗
+  |={⊤,∅}▷=> state_interp σ2 κs (pred (length t2)) ∗ WPC e2 @ s; ⊤; ∅ {{ Φ }} {{ Φc}}  ∗ wptp s t2'.
+Proof.
+  iIntros (Hstep) "Hσ He Ht".
+  destruct Hstep as [e1' σ1' e2' σ2' efs [|? t1'] t2' ?? Hstep]; simplify_eq/=.
+  - iExists e2', (t2' ++ efs). iModIntro. iSplitR; first by eauto.
+    iMod (wpc_step with "Hσ He") as "H"; first done.
+    iIntros "!> !>". iMod "H" as "(Hσ & He2 & Hefs)".
+    iIntros "!>". rewrite Nat.add_comm app_length. iFrame.
+  - iExists e, (t1' ++ e2' :: t2' ++ efs); iSplitR; first eauto.
+    iFrame "He". iDestruct "Ht" as "(Ht1 & He1 & Ht2)".
+    iModIntro. iMod (wpc_step with "Hσ He1") as "H"; first done.
+    iIntros "!> !>". iMod "H" as "(Hσ & He2 & Hefs)". iIntros "!>".
+    rewrite !app_length /= !app_length.
+    replace (length t1' + S (length t2' + length efs))
+      with (length efs + (length t1' + S (length t2'))) by omega. iFrame.
+Qed.
+
+Lemma wptp_steps s n e1 t1 κs κs' t2 σ1 σ2 Φ Φc :
+  nsteps n (e1 :: t1, σ1) κs (t2, σ2) →
+  state_interp σ1 (κs ++ κs') (length t1) -∗ WPC e1 @ s; ⊤; ∅ {{ Φ }} {{ Φc }} -∗ wptp s t1
+  ={⊤,∅}▷=∗^n ∃ e2 t2',
+    ⌜t2 = e2 :: t2'⌝ ∗
+    state_interp σ2 κs' (pred (length t2)) ∗
+    WPC e2 @ s; ⊤; ∅ {{ Φ }} {{ Φc }} ∗ wptp s t2'.
+Proof.
+  revert e1 t1 κs κs' t2 σ1 σ2; simpl.
+  induction n as [|n IH]=> e1 t1 κs κs' t2 σ1 σ2 /=.
+  { inversion_clear 1; iIntros "???"; iExists e1, t1; iFrame; eauto 10. }
+  iIntros (Hsteps) "Hσ He Ht". inversion_clear Hsteps as [|?? [t1' σ1']].
+  rewrite -(assoc_L (++)).
+  iMod (wptp_step with "Hσ He Ht") as (e1' t1'' ?) ">H"; first eauto; simplify_eq.
+  iIntros "!> !>". iMod "H" as "(Hσ & He & Ht)". iModIntro.
+  by iApply (IH with "Hσ He Ht").
+Qed.
+
+Lemma wpc_safe κs m e σ Φ Φc :
+  state_interp σ κs m -∗
+  WPC e {{ Φ }} {{ Φc }} ={⊤}=∗ ⌜is_Some (to_val e) ∨ reducible e σ⌝.
+Proof.
+  rewrite wpc_unfold /wpc_pre. iIntros "Hσ (H&_)".
+  destruct (to_val e) as [v|] eqn:?; first by eauto.
+  iSpecialize ("H" $! σ [] κs with "Hσ"). rewrite sep_elim_l.
+  iMod (fupd_plain_mask with "H") as %?; eauto.
+Qed.
+
+Lemma wptp_strong_adequacy Φ Φc κs' s n e1 t1 κs e2 t2 σ1 σ2 :
+  nsteps n (e1 :: t1, σ1) κs (t2, σ2) →
+  state_interp σ1 (κs ++ κs') (length t1) -∗
+  WPC e1 @ s; ⊤; ∅ {{ Φ }} {{ Φc }} -∗
+  wptp s t1 ={⊤,∅}▷=∗^(S n) (∃ e2 t2',
+    ⌜ t2 = e2 :: t2' ⌝ ∗
+    ⌜ ∀ e2, s = NotStuck → e2 ∈ t2 → (is_Some (to_val e2) ∨ reducible e2 σ2) ⌝ ∗
+    state_interp σ2 κs' (length t2') ∗
+    from_option Φ True (to_val e2) ∗
+    ([∗ list] v ∈ omap to_val t2', fork_post v)).
+Proof.
+  iIntros (Hstep) "Hσ He Ht". rewrite Nat_iter_S_r.
+  iDestruct (wptp_steps with "Hσ He Ht") as "Hwp"; first done.
+  iApply (step_fupdN_wand with "Hwp").
+  iDestruct 1 as (e2' t2' ?) "(Hσ & Hwp & Ht)"; simplify_eq/=.
+  iMod (fupd_plain_keep_l ⊤
+    ⌜ ∀ e2, s = NotStuck → e2 ∈ (e2' :: t2') → (is_Some (to_val e2) ∨ reducible e2 σ2) ⌝%I
+    (state_interp σ2 κs' (length t2') ∗ WPC e2' @ s; ⊤; ∅ {{ v, Φ v }} {{ Φc }} ∗ wptp s t2')%I
+    with "[$Hσ $Hwp $Ht]") as "(Hsafe&Hσ&Hwp&Hvs)".
+  { iIntros "(Hσ & Hwp & Ht)" (e' -> He').
+    apply elem_of_cons in He' as [<-|(t1''&t2''&->)%elem_of_list_split].
+    - iMod (wpc_safe with "Hσ Hwp") as "$"; auto.
+    - iDestruct "Ht" as "(_ & He' & _)". by iMod (wpc_safe with "Hσ He'"). }
+  iApply step_fupd_fupd. iApply step_fupd_intro; first done. iNext.
+  iExists _, _. iSplitL ""; first done. iFrame "Hsafe Hσ".
+  iSplitL "Hwp".
+  - destruct (to_val e2') as [v2|] eqn:He2'; last done.
+    apply of_to_val in He2' as <-. iApply (wpc_value_inv' with "Hwp").
+  - clear Hstep. iInduction t2' as [|e t2'] "IH"; csimpl; first by iFrame.
+    iDestruct "Hvs" as "[Hv Hvs]". destruct (to_val e) as [v|] eqn:He.
+    + apply of_to_val in He as <-. iMod (wpc_value_inv' with "Hv") as "$".
+      by iApply "IH".
+    + by iApply "IH".
+Qed.
+
+Lemma wptp_strong_crash_adequacy Φ Φc κs' s n e1 t1 κs e2 t2 σ1 σ2 :
+  nsteps n (e1 :: t1, σ1) κs (t2, σ2) →
+  state_interp σ1 (κs ++ κs') (length t1) -∗
+  WPC e1 @ s; ⊤; ∅ {{ Φ }} {{ Φc }} -∗
+  wptp s t1 ={⊤,∅}▷=∗^(S n) |={⊤, ∅}=> (∃ e2 t2',
+    ⌜ t2 = e2 :: t2' ⌝ ∗
+    Φc ∗ state_interp σ2 κs' (length t2')).
+Proof.
+  iIntros (Hstep) "Hσ He Ht". rewrite Nat_iter_S_r.
+  iDestruct (wptp_steps with "Hσ He Ht") as "Hwp"; first done.
+  iApply (step_fupdN_wand with "Hwp").
+  iDestruct 1 as (e2' t2' ?) "(Hσ & Hwp & Ht)"; simplify_eq/=.
+  iMod (fupd_plain_keep_l ⊤
+    ⌜ ∀ e2, s = NotStuck → e2 ∈ (e2' :: t2') → (is_Some (to_val e2) ∨ reducible e2 σ2) ⌝%I
+    (state_interp σ2 κs' (length t2') ∗ WPC e2' @ s; ⊤; ∅ {{ v, Φ v }} {{ Φc }} ∗ wptp s t2')%I
+    with "[$Hσ $Hwp $Ht]") as "(Hsafe&Hσ&Hwp&Hvs)".
+  { iIntros "(Hσ & Hwp & Ht)" (e' -> He').
+    apply elem_of_cons in He' as [<-|(t1''&t2''&->)%elem_of_list_split].
+    - iMod (wpc_safe with "Hσ Hwp") as "$"; auto.
+    - iDestruct "Ht" as "(_ & He' & _)". by iMod (wpc_safe with "Hσ He'"). }
+  iApply step_fupd_fupd. iApply step_fupd_intro; first done. iNext.
+  iModIntro. iExists _, _.
+  rewrite {1}wpc_unfold /wpc_pre.
+  iDestruct "Hwp" as "(_&Hwp)".
+  iMod ("Hwp" with "[$]") as "($&$)".
+  iModIntro; eauto.
+Qed.
+End crash_adequacy.
+
+(*** Recovery ***)
 
 Class pbundleG (T: ofeT) := {
   pbundleT : T
@@ -13,13 +153,13 @@ Class perennialG (Λ : language) (CS: crash_semantics Λ) (T: ofeT) (Σ : gFunct
 }.
 
 Definition wpr_pre `{perennialG Λ CS T Σ} (s : stuckness)
-    (wpr : pbundleG T -d> coPset -d> expr Λ -d> expr Λ -d> (val Λ -d> iPropO Σ) -d> iPropO Σ -d> iPropO Σ) :
-  pbundleG T -d> coPset -d> expr Λ -d> expr Λ -d> (val Λ -d> iPropO Σ) -d> iPropO Σ -d> iPropO Σ :=
+    (wpr : pbundleG T -d> coPset -d> expr Λ -d> expr Λ -d> (val Λ -d> iPropO Σ) -d> (pbundleG T -d> iPropO Σ) -d> iPropO Σ) :
+  pbundleG T -d> coPset -d> expr Λ -d> expr Λ -d> (val Λ -d> iPropO Σ) -d> (pbundleG T -d> iPropO Σ) -d> iPropO Σ :=
   λ t E e rec Φ Φr,
   (WPC e @ s ; E ; ∅
      {{ Φ }}
      {{ ∀ σ σ' (HC: crash_prim_step CS σ σ') κs n,
-        state_interp σ κs n ={∅}=∗  ▷ ∃ t, state_interp σ' [] 0 ∗ wpr t E rec rec (λ _, Φr) Φr }})%I.
+        state_interp σ κs n ={∅}=∗  ▷ ∃ t, state_interp σ' [] 0 ∗ wpr t E rec rec (λ _, Φr t) (λ t', Φr t')}})%I.
 
 Local Instance wpr_pre_contractive `{!perennialG Λ CS T Σ} s : Contractive (wpr_pre s).
 Proof.
@@ -28,7 +168,7 @@ Proof.
 Qed.
 
 Definition wpr_def `{!perennialG Λ CS T Σ} (s : stuckness) :
-  pbundleG T → coPset → expr Λ → expr Λ → (val Λ → iProp Σ) → iProp Σ → iProp Σ := fixpoint (wpr_pre s).
+  pbundleG T → coPset → expr Λ → expr Λ → (val Λ → iProp Σ) → (pbundleG T → iProp Σ) → iProp Σ := fixpoint (wpr_pre s).
 Definition wpr_aux `{!perennialG Λ CS T Σ} : seal (@wpr_def Λ CS T Σ _). by eexists. Qed.
 Definition wpr `{!perennialG Λ CS T Σ} := wpr_aux.(unseal).
 Definition wpr_eq `{!perennialG Λ CS T Σ} : wpr = @wpr_def Λ CS T Σ _ := wpr_aux.(seal_eq).
@@ -38,7 +178,7 @@ Context `{!perennialG Λ CS T Σ}.
 Implicit Types s : stuckness.
 Implicit Types P : iProp Σ.
 Implicit Types Φ : val Λ → iProp Σ.
-Implicit Types Φc : iProp Σ.
+Implicit Types Φc : pbundleG T → iProp Σ.
 Implicit Types v : val Λ.
 Implicit Types e : expr Λ.
 
@@ -49,7 +189,7 @@ Proof. rewrite wpr_eq. apply (fixpoint_unfold (wpr_pre s)). Qed.
 (* There's a stronger version of this *)
 Lemma wpr_strong_mono s t E e rec Φ Ψ Φr Ψr :
   wpr s t E e rec Φ Φr -∗
-  (∀ v, Φ v ==∗ Ψ v) ∧ (Φr ==∗ Ψr) -∗
+  (∀ v, Φ v ==∗ Ψ v) ∧ (∀ t, Φr t ==∗ Ψr t) -∗
   wpr s t E e rec Ψ Ψr.
 Proof.
   iIntros "H HΦ". iLöb as "IH" forall (e t E Φ Ψ Φr Ψr).
@@ -57,22 +197,21 @@ Proof.
   iApply (wpc_strong_mono with "H") ; auto.
   iSplit.
   { iDestruct "HΦ" as "(H&_)". iIntros. iMod ("H" with "[$]"); eauto. }
-  iIntros "H". 
+  iIntros "H".
   iModIntro. iIntros (?????) "Hinterp". iMod ("H" with "[//] Hinterp") as "H".
   iModIntro. iNext. iDestruct "H" as (?) "(?&H)".
   iExists _. iFrame. iApply ("IH" with "[$]").
   iSplit; iIntros; iDestruct ("HΦ") as "(_&H)"; by iMod ("H" with "[$]").
 Qed.
 
-(* To prove a recovery wp for e with rec, it suffices to prove a crash wp for e, where the crash
-   condition implies the precondition for a crash wp for rec *)
-(* XXX the second predicate for wpr should take t as an argument, so we don't have this existential *)
+(* To prove a recovery wp for e with rec, it suffices to prove a crash wp for e,
+   where the crash condition implies the precondition for a crash wp for rec *)
 Lemma idempotence_wpr s E e rec Φx Φrx Φcx t:
   ((WPC e @ s ; E ; ∅ {{ Φx t }} {{ Φcx t }}) -∗
    (□ ∀ (t: pbundleG T) σ σ' (HC: crash_prim_step CS σ σ') κs n,
         Φcx t -∗ state_interp σ κs n ={∅}=∗
         ▷ ∃ t', state_interp σ' [] 0 ∗ WPC rec @ s ; E ; ∅ {{ (λ _, Φrx t') }} {{ Φcx t' }}) -∗
-    wpr s t E e rec (Φx t) (∃ t', Φrx t'))%I.
+    wpr s t E e rec (Φx t) Φrx)%I.
 Proof.
   iLöb as "IH" forall (E e t Φx).
   iIntros "He #Hidemp".
@@ -83,19 +222,9 @@ Proof.
   { eauto. }
   iModIntro. iNext. iDestruct "H" as (t') "(?&Hc)".
   iExists _. iFrame.
-  iApply ("IH" $! E rec t' (λ t _, ∃ t', Φrx t')%I with "[Hc]").
+  iApply ("IH" $! E rec t' (λ t _, Φrx t)%I with "[Hc]").
   { iApply (wpc_strong_mono with "Hc"); auto. }
   eauto.
 Qed.
 
-(*
-Definition recv_idemp Σ {Λ CS} `{!invPreG Σ} s (rec: expr Λ) φinv φrec :=
-  (□ (∀ `{Hinv : invG Σ} σ1 σ1' κs (Hcrash: crash_prim_step CS σ1 σ1'),
-        (φinv σ1 ={⊤}=∗
-           ∃ (stateI : state Λ → list (observation Λ) → nat → iProp Σ)
-             (fork_post : val Λ → iProp Σ),
-             let _ : irisG Λ Σ := IrisG _ _ Hinv stateI fork_post in
-             stateI σ1' κs 0 ∗
-             wp_crash s ⊤ rec (λ _, ∀ σ n, stateI σ [] n ={⊤, ∅}=∗ φrec σ ) φinv)))%I.
-
-*)
+End wpr.
